proving reflexivity

src/coq_formalism/simulation.v
@@ -7,20 +7,19 @@
     By: Anna Fritz
     Date: August 2, 2023 *)
 
-    Set Implicit Arguments.
+Require Import Coq.Relations.Relation_Definitions.
+Set Implicit Arguments.
 
-
-Inductive sl := 
-| silentlabel.
+Context {label L: Set}.  
 
 (* First, define Labeled Transition System
  * Given a set of states and labels, 
  * define a transition relation and initial state.
  * A label may either be a label or the silent label.  *)
 
-Record LTS (state label : Type) : Type := {
-    initial : state -> Prop;
-    step : state -> label + sl -> state -> Prop 
+Record LTS (state : Type) : Type := {
+    initial : state;
+    step : state -> label -> state -> Prop 
 }.
 
 Check LTS.
@@ -30,20 +29,91 @@ Definition relation (X : Type) := X -> X -> Prop.
 
 (* bisimilarity relation for two states 
 * type of this relation should be state -> state -> Prop *)
-Definition BR_state {state label} (sys : LTS state label) (R: relation state) : Prop := 
+Definition BR_state {state} (sys : LTS state) (R: relation state) : Prop := 
     forall q p, R q p /\ forall l q', (sys.(step) q l q') -> 
     (exists p', (sys.(step) p l p') /\ R q' p').
 
 (* simulation is one way *)
-Definition simulation {state label} (S1 S2 : LTS state label) (R : relation state) : Prop := 
+Definition simulation {state} (S1 S2 : LTS state) (R : relation state) : Prop := 
     forall q p, R q p /\ forall q' l, S1.(step) q l q' -> 
     exists p', (S2.(step) p l p') /\ R q' p'.
 
-Definition bisimulation {state label} (S1 S2 : LTS state label) (R : relation state) : Prop := 
+(* strong bisimulation is two way *)
+Definition bisimulation {state1 state2} (S1: LTS state1) (S2: LTS state2) (R : state1 -> state2 -> Prop) : Prop := 
+    R S1.(initial) S2.(initial) /\
     ( forall q p, R q p /\ forall q' l, S1.(step) q l q' -> 
     exists p', (S2.(step) p l p') /\ R q' p' ) /\
     ( forall q p, R q p /\ forall p' l, S2.(step) p l p' -> 
     exists q', (S1.(step) q l q') /\ R q' p').
+
+ 
+(* Redefine Label transition system to include silent labels *)
+
+Inductive sl := 
+| silentlabel.
+
+Record LTS' := {
+    st : Set ; 
+    inital : st -> Prop ; 
+    step' : st -> st -> Prop ;
+    l : st -> L + sl
+  }.
+
+(* the transitive reflexive closure of silent transitions *)
+Inductive silentstar (lts : LTS') : lts.(st) -> lts.(st) -> Prop := 
+| star_refl : forall (s : lts.(st)), silentstar lts s s
+| star_trans : forall (s s' s'' : lts.(st)), lts.(step') s s' -> 
+                lts.(l) s = inr silentlabel -> 
+                silentstar lts s' s'' ->  silentstar lts s s''.
+
+(* Defining a weak simulation. This is a one-way relation between two LTS'.
+ * There are three cases.  *)
+Definition weakSimulation (S1 S2 : LTS') (R: S1.(st) -> S2.(st) -> Prop) := 
+    (* inital condition. All start states in one graph must be present in the other. *)
+    (forall (s : S1.(st)), S1.(inital) s -> 
+    exists (r : S2.(st)), R s r /\ S1.(l) s = S2.(l) r) /\ 
+
+    (* if there is a silent step in S1 then there exists some related silent step in S2 *)
+    ( forall p q, R p q -> forall p', S1.(step') p p' /\ S1.(l) p = inr silentlabel  -> 
+    exists q', silentstar S2 q q' /\ R p' q') /\ 
+    
+    (* if there is some labeled step in S1 then there exists some labeled transition in S2 that may include silent states *)
+    (forall p q, R p q -> forall p' a, S1.(step') p p' /\ S1.(l) p = inl a -> 
+     exists q1 q2 q', silentstar S2 q q1 /\ S2.(step') q1 q2 /\ S2.(l) q1 = inl a /\ silentstar S2 q2 q' /\ R p' q'). 
+
+Notation "x <= y" := (weakSimulation x y) (at level 70).
+
+(* Prove that a weak simulation is reflexive *)
+Lemma  WS_refl : forall x, exists r , (x <= x) r.
+Proof.
+    intros. exists eq. 
+    unfold weakSimulation. split.
+    + intros. exists s; eauto.
+    + split.
+    ++ intros. exists p'. split; eauto.
+    +++ apply star_trans with (s' := p'); try (rewrite <- H; destruct H0 as [H0 H1]; eauto). apply star_refl.
+    ++ intros. exists p. exists p'. exists p'; repeat split.
+    +++ rewrite H. apply star_refl.
+    +++ inversion H0; eauto.
+    +++ inversion H0; eauto.
+    +++ apply star_refl.         
+Qed. 
+
+Lemma  WB_trans : forall x y z,       
+                    ( exists r1, weakBisimulation x y r1 ) -> 
+                    ( exists r2, weakBisimulation y z r2 ) -> 
+                      exists r3, weakBisimulation x z r3.
+Proof. Admitted. 
+
+(* need to define equal... maybe isomorphism as equivalence ...? *)
+
+Lemma WB_antisym : forall x y, 
+                    ( exists r1, weakBisimulation x y r1 ) -> 
+                    ( exists r2, weakBisimulation y x r2 ) -> 
+                      x = y.
+
+
+
 
 
 
@@ -53,5 +123,5 @@ Inductive trc {A} (R : A -> A -> Prop) : A -> A -> Prop :=
 | TrcTrans : forall x y z, R x y -> trc R y z -> trc R x z.
 
 (* Might be useful to define reachable states *)
-Inductive reachable {state label} (sys : LTS state label) (st : state) : Prop :=
-| Reachable : forall st0, sys.(initial) st0 -> trc sys.(step) st0 st -> reachable sys st.
+Inductive reachable {state} (sys : LTS state) (st : state) : Prop :=
+| Reachable : forall st0, sys.(initial) st0 -> trc sys.(step) st0 _ st -> reachable sys st.
